Veritas.SeqAux.fst
@@ -524,3 +524,33 @@ let rec reduce_aux (#a:Type) (#b:Type) (b0: b) (f: a -> b -> b) (s: seq a):
     f e b' 
 
 let reduce = reduce_aux
+
+let lemma_reduce_empty (#a:Type) (#b:eqtype) (b0:b) (f:a -> b -> b):
+  Lemma (reduce b0 f (empty #a) = b0) = ()
+
+let rec lemma_reduce_prefix_aux (#a:Type) (#b:eqtype) (b0: b) (f: a -> b -> b) (s: seq a) (i: seq_index s):
+  Lemma (requires True)
+        (ensures (reduce b0 f s = reduce (reduce b0 f (prefix s i)) f (suffix s (length s - i))))
+        (decreases (length s)) = 
+  let n = length s in
+  if n = 0 then ()
+  else 
+    let s' = prefix s (n - 1) in
+    let b' = reduce b0 f s' in
+    let e = index s (n - 1) in
+    if i = n - 1 then ()
+    else 
+      lemma_reduce_prefix_aux b0 f s' i
+
+let lemma_reduce_prefix = lemma_reduce_prefix_aux
+
+let rec lemma_reduce_identity_aux (#a:Type) (#b:eqtype) (b0: b) (f: a -> b -> b) (s: seq a):
+  Lemma (requires (forall (x:a). f x b0 = b0))
+        (ensures (reduce b0 f s = b0))
+        (decreases (length s)) = 
+  let n = length s in
+  if n = 0 then ()
+  else 
+    lemma_reduce_identity_aux b0 f (prefix s (n - 1))
+
+let lemma_reduce_identity = lemma_reduce_identity_aux
